progress, but case rec is actually very administrative

theories/Confluence.v
@@ -61,8 +61,8 @@ Inductive ortho_red : ctx -> level -> term -> term → term → Prop :=
 | ortho_rec : 
     ∀ Γ l P p_zero p_succ t P' p_zero' p_succ' t',
       Γ ,, (ty 0 , Nat) ⊢< Ax l > P ⟹ P' : Sort l ->
-      Γ ⊢< l > p_zero ⟹ p_zero' : P <[ p_zero .. ] -> 
-      Γ ,, (ty 0 , Nat) ,, (l , P <[ (var 0) .. ]) ⊢< l > p_succ ⟹ p_succ' : P <[ (succ (var 0)) .. ] ->
+      Γ ⊢< l > p_zero ⟹ p_zero' : P <[ zero .. ] -> 
+      Γ ,, (ty 0 , Nat) ,, (l , P) ⊢< l > p_succ ⟹ p_succ' : P <[ (succ (var 1)) .: (shift >> (shift >> var)) ]  ->
       Γ ⊢< ty 0 > t ⟹ t' : Nat ->
       Γ ⊢< l > rec l P p_zero p_succ t ⟹ rec l P' p_zero' p_succ' t' : P <[ t .. ]
   
@@ -99,15 +99,15 @@ Inductive ortho_red : ctx -> level -> term -> term → term → Prop :=
 | ortho_rec_zero : 
     ∀ Γ l P p_zero p_succ p_zero',
       Γ ,, (ty 0 , Nat) ⊢< Ax l > P : Sort l ->
-      Γ ⊢< l > p_zero ⟹ p_zero' : P <[ p_zero .. ] -> 
-      Γ ,, (ty 0 , Nat) ,, (l , P <[ (var 0) .. ]) ⊢< l > p_succ : P <[ (succ (var 0)) .. ] ->
+      Γ ⊢< l > p_zero ⟹ p_zero' : P <[ zero .. ] -> 
+      Γ ,, (ty 0 , Nat) ,, (l , P) ⊢< l > p_succ : P <[ (succ (var 1)) .: (shift >> (shift >> var)) ]  ->
       Γ ⊢< l > rec l P p_zero p_succ zero ⟹ p_zero' : P <[ zero .. ]
 
 | ortho_rec_succ : 
     ∀ Γ l P p_zero p_succ t P' p_zero' p_succ' t',
       Γ ,, (ty 0 , Nat) ⊢< Ax l > P ⟹ P' : Sort l ->
-      Γ ⊢< l > p_zero ⟹ p_zero' : P <[ p_zero .. ] -> 
-      Γ ,, (ty 0 , Nat) ,, (l , P <[ (var 0) .. ]) ⊢< l > p_succ ⟹ p_succ' : P <[ (succ (var 0)) .. ] ->
+      Γ ⊢< l > p_zero ⟹ p_zero' : P <[ zero .. ] -> 
+      Γ ,, (ty 0 , Nat) ,, (l , P) ⊢< l > p_succ ⟹ p_succ' : P <[ (succ (var 1)) .: (shift >> (shift >> var)) ]  ->
       Γ ⊢< ty 0 > t ⟹ t' : Nat ->
       Γ ⊢< l > rec l P p_zero p_succ (succ t) ⟹ 
           p_succ' <[ t' .: (rec l P' p_zero' p_succ' t') ..] : P <[ (succ t) .. ]
@@ -119,9 +119,9 @@ where "Γ ⊢< l > t ⟹ u : A" := (ortho_red Γ l t u A).
 Reserved Notation "Γ ⊢s σ ⟹ τ : Δ" (at level 50, σ, τ, Δ at next level).
 
 Inductive ortho_subst (Γ : ctx) : ctx -> (nat -> term) -> (nat -> term) -> Prop :=
-  | well_sempty (σ σ' : nat -> term) : 
+  | ortho_sempty (σ σ' : nat -> term) : 
     Γ ⊢s σ ⟹ σ' : ∙
-  | well_scons (σ σ' : nat -> term) (Δ : ctx) l (A : term) :
+  | ortho_scons (σ σ' : nat -> term) (Δ : ctx) l (A : term) :
     Γ ⊢s (↑ >> σ) ⟹ (↑ >> σ') : Δ ->
     Γ ⊢< l > σ var_zero ⟹ σ' var_zero : A <[↑ >> σ] ->
     Γ ⊢s σ ⟹ σ' : (Δ ,, (l , A)) 
@@ -255,15 +255,22 @@ Lemma ortho_app_inv Γ i l1 l2 A1 B1 t u w T :
   )).
 Admitted.
 
+
+Require Import Stdlib.Program.Equality.
+
 Lemma ortho_nat_inv Γ l' t A :
   Γ ⊢< l' > Nat ⟹ t : A → t = Nat.
 Proof.
-Admitted.
+  intros.
+  dependent induction H; eauto. dependent induction H. apply IHtyping; eauto. eapply type_conv; eauto using conv_sym.
+Qed.
 
 Lemma ortho_zero_inv Γ l' t A :
   Γ ⊢< l' > zero ⟹ t : A → t = zero.
 Proof.
-Admitted.
+  intros.
+  dependent induction H; eauto. dependent induction H. apply IHtyping; eauto. eapply type_conv; eauto using conv_sym.
+Qed.
 
 Lemma ortho_succ_inv Γ l' t n A :
   Γ ⊢< l' > succ n ⟹ t : A → 
@@ -271,10 +278,38 @@ Lemma ortho_succ_inv Γ l' t n A :
     t = succ n' /\
     Γ ⊢< ty 0 > n ⟹ n' : Nat.
 Proof.
-Admitted.
+  intros.
+  dependent induction H; eauto. dependent induction H. apply IHtyping; eauto. eapply type_conv; eauto using conv_sym.
+Qed.
 
-
-
+Lemma ortho_rec_inv Γ i l P p_zero p_succ u t T :
+  Γ ⊢< ty i > rec l P p_zero p_succ u ⟹ t : T →
+  ( (* by rec cong *)
+    exists P' p_zero' p_succ' u',
+      t = rec l P' p_zero' p_succ' u' ∧
+      Γ ,, (ty 0, Nat) ⊢< Ax l > P ⟹ P' : Sort l ∧
+      Γ ⊢< l > p_zero ⟹ p_zero' : P <[ zero ..] ∧
+      Γ ,, (ty 0, Nat) ,, (l, P) ⊢< l > p_succ ⟹ p_succ' : P <[ (succ (var 1)) .: (shift >> (shift >> var)) ]  ∧
+      Γ ⊢< ty 0 > u ⟹ u' : Nat
+  ) \/ ( (* by ortho_zero *)
+    exists p_zero',
+      t = p_zero' ∧ u = zero ∧
+      Γ ⊢< l > p_zero ⟹ p_zero' : P <[ zero ..]
+  ) \/ ( (* by ortho_succ *)
+    exists P' p_zero' p_succ' n n',
+      t = p_succ' <[ n' .: (rec l P' p_zero' p_succ' n') ..] ∧ u = succ n ∧
+      Γ ,, (ty 0, Nat) ⊢< Ax l > P ⟹ P' : Sort l ∧
+      Γ ⊢< l > p_zero ⟹ p_zero' : P <[ zero ..] ∧
+      Γ ,, (ty 0, Nat) ,, (l, P) ⊢< l > p_succ ⟹ p_succ' : P <[ (succ (var 1)) .: (shift >> (shift >> var)) ]   ∧
+      Γ ⊢< ty 0 > n ⟹ n' : Nat).
+Proof.
+  intros.
+  dependent induction H.
+  - left. do 4 eexists. split. reflexivity. eauto. 
+  - eapply IHortho_red. eauto. eauto.
+  - right. left. eauto.
+  - right. right. do 5 eexists. split. reflexivity. split. reflexivity. eauto.
+Qed.
 
 (* TODO finish *)
 
@@ -290,7 +325,7 @@ Ltac ttinv h :=
     | Nat => eapply ortho_nat_inv in h
     | zero => eapply ortho_zero_inv in h
     | succ _ => eapply ortho_succ_inv in h
-    | _ => h
+    | rec _ _ _ _ _ => eapply ortho_rec_inv in h
     end
   end.
 
@@ -360,18 +395,39 @@ Proof.
   - apply (ortho_diamond_prop _ _ _ _ _ H1 H2).
 Qed.
 
-(* 
-Lemma ortho_diamond_app_beta : 
-  Γ ⊢< _ > A ≡ A' : (Sort l1) -> 
-  Γ ,, (l1 , A) ⊢< _ > B ≡ B' : (Sort l2) -> 
-  
-  Γ ,, (l1 , A) ⊢< _ > u ⟹ u' : B -> 
-  Γ ⊢< _ > v ⟹ v' : A ->
-  
-  Γ ,, (l1 , A') ⊢< _ > u ⟹ u' : B' -> 
-  Γ ⊢< _ > v ⟹ v' : A ->
-   *)
 
+
+Ltac ctx_conv_auto := 
+  match goal with 
+  (* | H : ?Γ ⊢< ?l > ?t ⟹ ?u : ?A |- ⊢ ?Γ ≡ ?Γ => eapply refl_ctx; eauto using H, ortho_validity, validity_ty
+  | H : ?Γ ⊢< ?l > ?t : ?A |- ⊢ ?Γ ≡ ?Γ => eapply refl_ctx; eauto using H, validity_ty
+  | H : ?Γ ⊢< ?l > ?t ≡ ?u : ?A |- ⊢ ?Γ ≡ ?Γ => eapply refl_ctx; eauto using H, ortho_validity, validity_conv, validity_ty
+  | H : ⊢ ?Γ |- ⊢ ?Γ ≡ ?Γ => eapply refl_ctx; eauto using H
+   
+   *)
+  | |- ⊢ ?Γ,, (?l, ?A) ≡ ?Γ,, (?l, ?B) =>
+    apply conv_ccons; [ (eapply refl_ctx; eauto using ctx_cons, ctx_nil, type_nat) | eauto using ortho_to_conv, conv_sym, conv_trans ]
+  end.
+
+
+Ltac use_auto :=
+  match goal with
+  (* | H : ?Γ ⊢< ?l > ?t ⟹ ?u : ?A |- ?Γ ⊢< ?l > ?t ⟹ ?u : ?A => exact H *)
+  | H : ?Γ ⊢< ?l > ?t ⟹ ?u : ?A |- ?Δ ⊢< ?l > ?t ⟹ ?u : ?A =>
+    apply (ortho_conv_in_ctx Γ Δ l t u A); [ ctx_conv_auto | exact H]
+  | H : ?Γ ⊢< ?l > ?t ⟹ ?u : ?A |- ?Γ ⊢< ?l > ?t ⟹ ?u : ?B =>
+    apply (ortho_conv Γ l A B t u); [exact H | idtac]
+  | H : ?Γ ⊢< ?l > ?t ⟹ ?u : ?A |- ?Δ ⊢< ?l > ?t ⟹ ?u : ?B =>
+    apply (ortho_conv_in_ctx Γ Δ l t u B); [ ctx_conv_auto | apply (ortho_conv Γ l A B t u); [exact H | eauto using ortho_to_conv, conv_sym, conv_trans]]
+  | H : ?Γ ⊢< ?l > ?t : ?A |- ?Δ ⊢< ?l > ?t : ?B =>
+    apply (conv_in_ctx_ty Γ Δ l t B); [ ctx_conv_auto | apply (type_conv Γ l A B t); [exact H | eauto using ortho_to_conv, conv_sym, conv_trans]]
+  (* | H : ?Γ ⊢< ?l > ?t ≡ ?u : ?A |- H : ?Γ ⊢< ?l > ?t ≡ ?u : ?A *)
+  | H : ?Γ ⊢< ?l > ?t ≡ ?u : ?A |- ?Δ ⊢< ?l > ?t ≡ ?u : ?A => 
+    apply (conv_in_ctx_conv Γ Δ l t u A); [ ctx_conv_auto | exact H]
+  | H : ?Γ ⊢< ?l > ?t ≡ ?u : ?A |- ?Δ ⊢< ?l > ?u ≡ ?t : ?A => 
+    apply conv_sym; apply (conv_in_ctx_conv Γ Δ l t u A); [ ctx_conv_auto | exact H]
+  | |- _ => idtac
+  end.
 
 (* TODO: think of some nice tactics to make the easy cases of the proof more direct *)
 
@@ -413,18 +469,10 @@ Proof.
     ttinv t_red_t''. destruct t_red_t'' as (A'' & B'' & t''_eq_pi & _ & A_red_A'' & B_red_B'' & _). 
     rewrite t''_eq_pi in *. clear t''_eq_pi t''.
 
-    epose proof (IH_A := IH _ _ _ _ _ _ _ A_red_A' A_red_A''). destruct IH_A as (A''' & A'_red_A''' & A''_red_A'''). 
-    shelve. Unshelve. simpl. lia.
-    epose proof (IH_B := IH _ _ _ _ _ _ _ B_red_B' B_red_B''). destruct IH_B as (B''' & B'_red_B''' & B''_red_B'''). 
-    shelve. Unshelve. simpl. lia.
-
+    epose proof (IH_A := IH A ltac:(simpl; lia) _ _ _ _ _ A_red_A' A_red_A''). destruct IH_A as (A''' & A'_red_A''' & A''_red_A'''). 
+    epose proof (IH_B := IH B ltac:(simpl; lia) _ _ _ _ _ B_red_B' B_red_B''). destruct IH_B as (B''' & B'_red_B''' & B''_red_B''').
     do 4 eexists. exists (Pi l l0 A''' B'''). 
-
-    split; apply ortho_pi; auto.
-    (* todo: how to optimise this?*)
-    + eapply ortho_conv_in_ctx. apply conv_ccons. eapply refl_ctx. auto. eauto using ortho_to_conv. auto.
-    + eapply ortho_conv_in_ctx. apply conv_ccons. eapply refl_ctx. auto. eauto using ortho_to_conv. auto.
-    
+    split; apply ortho_pi; eauto; use_auto.
 
   (* lam *)
   - rename t1 into A. rename t2 into B. rename t3 into u.
@@ -433,99 +481,54 @@ Proof.
     ttinv t_red_t''. destruct t_red_t'' as (A'' & B'' & u'' & _ & _ & t''_eq_lam & A_conv_A'' & B_conv_B'' & u_red_u'').
     rewrite t''_eq_lam in *. clear t''_eq_lam t''.
 
-    epose proof (IH_u := IH _ _ _ _ _ _ _ u_red_u' u_red_u''). destruct IH_u as (u''' & u'_red_u''' & u''_red_u'''). 
-    shelve. Unshelve. simpl. lia.
+    epose proof (IH_u := IH u ltac:(simpl; lia) _ _ _ _ _ u_red_u' u_red_u''). destruct IH_u as (u''' & u'_red_u''' & u''_red_u'''). 
 
-    do 4 eexists. exists (lam l l0 A B u'''). split; apply ortho_lam; eauto using conv_sym. 
-    + eapply (conv_in_ctx_conv (Γ,, (l, _))). apply conv_ccons. eapply refl_ctx. auto. eauto using ortho_to_conv. auto using conv_sym.
-    + eapply (ortho_conv_in_ctx (Γ,, (l, _))). apply conv_ccons. eapply refl_ctx. auto. eauto using ortho_to_conv. auto using conv_sym.
-      eapply ortho_conv. eauto. eauto.
-    + eapply (conv_in_ctx_conv (Γ,, (l, _))). apply conv_ccons. eapply refl_ctx. auto. eauto using ortho_to_conv. auto using conv_sym.
-    + eapply (ortho_conv_in_ctx (Γ,, (l, _))). apply conv_ccons. eapply refl_ctx. auto. eauto using ortho_to_conv. auto using conv_sym.
-      eapply ortho_conv. eauto. eauto.
-
+    do 4 eexists. exists (lam l l0 A B u'''). split; apply ortho_lam; eauto using conv_sym; use_auto.
 
   (* app *)
   - rename t1 into A. rename t2 into B. rename t3 into u. rename t4 into v.
-    ttinv t_red_t'. destruct t_red_t' as (i_eq & _ & [ t_red_t' | t_red_t' ]);
-    ttinv t_red_t''; destruct t_red_t'' as (_ & _ & [ t_red_t'' | t_red_t'' ]).
+    ttinv t_red_t'. destruct t_red_t' as (i_eq & _ & [ (A' & B' & u' & v' & t'_eq & A_conv_A' & B_conv_B' & u_red_u' & v_red_v') 
+                                                     | (A0 & B0 & w & w' & v' & u_eq & _ & _ & w_red_w' & v_red_v' & t'_eq) ]);
+    ttinv t_red_t''; destruct t_red_t'' as (_ & _ & [ (A'' & B'' & u'' & v'' & t''_eq & A_conv_A'' & B_conv_B'' & u_red_u'' & v_red_v'') 
+                                                    | (A0_ & B0_ & w_ & w'' & v'' & u_eq_ & A_conv_A0_ & B_conv_B0_ & w_red_w'' & v_red_v'' & t''_eq) ]);
+    try rewrite t'_eq in *; clear t'_eq t'; rewrite t''_eq in *; clear t''_eq t'';
+    try epose proof (IH_u := IH u ltac:(simpl; lia) _ _ _ _ _ u_red_u' u_red_u''); try destruct IH_u as (u''' & u'_red_u''' & u''_red_u'''); 
+    try epose proof (IH_v := IH v ltac:(simpl; lia) _ _ _ _ _ v_red_v' v_red_v''); try destruct IH_v as (v''' & v'_red_v''' & v''_red_v''').
+     
     (* app-cong x app-cong *)
-    + destruct t_red_t' as (A' & B' & u' & v' & t'_eq & A_conv_A' & B_conv_B' & u_red_u' & v_red_v').
-      rewrite t'_eq in *. clear t'_eq t'.
-      destruct t_red_t'' as (A'' & B'' & u'' & v'' & t''_eq & A_conv_A'' & B_conv_B'' & u_red_u'' & v_red_v'').
-      rewrite t''_eq in *. clear t''_eq t''.
-
-      epose proof (IH_u := IH _ _ _ _ _ _ _ u_red_u' u_red_u''). destruct IH_u as (u''' & u'_red_u''' & u''_red_u'''). 
-      shelve. Unshelve. simpl. lia.
-      epose proof (IH_v := IH _ _ _ _ _ _ _ v_red_v' v_red_v''). destruct IH_v as (v''' & v'_red_v''' & v''_red_v'''). 
-      shelve. Unshelve. simpl. lia.
-
-      do 4 eexists. exists (app l l0 A B u''' v'''). split; apply ortho_app; eauto using conv_sym.
-      ++ eapply conv_in_ctx_conv. apply conv_ccons. eapply refl_ctx. auto. eauto using ortho_to_conv. auto using conv_sym.
-      ++ eapply ortho_conv. eauto. apply conv_pi; eauto.
-      ++ eapply ortho_conv. eauto. auto.
-      ++ eapply conv_in_ctx_conv. apply conv_ccons. eapply refl_ctx. auto. eauto using ortho_to_conv. auto using conv_sym.
-      ++ eapply ortho_conv. eauto. apply conv_pi; eauto.
-      ++ eapply ortho_conv. eauto. auto.
+    + do 4 eexists. exists (app l l0 A B u''' v'''). split; apply ortho_app; eauto using conv_sym; use_auto; eauto; apply conv_pi; eauto.
 
     (* app-cong x beta *)
-    + destruct t_red_t' as (A' & B' & u' & v' & t'_eq & A_conv_A' & B_conv_B' & u_red_u' & v_red_v').
-      rewrite t'_eq in *. clear t'_eq t'.
-      destruct t_red_t'' as (A0 & B0 & w & w'' & v'' & u_eq & A_conv_A0 & B_conv_B0 & w_red_w'' & v_red_v'' & t''_eq).
-      rewrite t''_eq. clear t''_eq t''.
-      
+    + rename u_eq_ into u_eq. rename w_ into w. rename A0_ into A0. rename B0_ into B0. rename A_conv_A0_ into A_conv_A0. rename B_conv_B0_ into B_conv_B0.
+
       rewrite u_eq in *. clear u_eq u. rewrite <- i_eq in *. clear l0 i_eq. 
 
       ttinv u_red_u'. destruct u_red_u' as (A0' & B0' & w' & _ & _ & u'_eq & A0_conv_A0' & B0_conv_B0' & w_red_w').
 
       rewrite u'_eq in *. clear u'_eq u'.
       
-      rename w_red_w' into _w_red_w'.
-      assert (Γ,, (l, A) ⊢< ty i > w ⟹ w' : B) as w_red_w'. 
-      { eapply ortho_conv. eapply ortho_conv_in_ctx. apply conv_ccons. eapply refl_ctx. auto. 
-        apply conv_sym. apply A_conv_A0. apply _w_red_w'. auto using conv_sym. }
-      clear _w_red_w'.
+      rename w_red_w' into temp. assert (Γ,, (l, A) ⊢< ty i > w ⟹ w' : B) as w_red_w'. {use_auto. use_auto. } clear temp.
+      rename B0_conv_B0' into temp. assert (Γ,, (l, A) ⊢< Ax (ty i) > B0 ≡ B0' : Sort (ty i)) as B0_conv_B0'.  {use_auto. } clear temp.
 
-      rename B0_conv_B0' into _B0_conv_B0'.
-      assert (Γ,, (l, A) ⊢< Ax (ty i) > B0 ≡ B0' : Sort (ty i)) as B0_conv_B0'. 
-      { eapply conv_in_ctx_conv. apply conv_ccons. eapply refl_ctx. auto. apply conv_sym. apply A_conv_A0. auto. }
-      clear _B0_conv_B0'.
-
-      epose proof (IH_w := IH _ _ _ _ _ _ _ w_red_w' w_red_w''). destruct IH_w as (w''' & w'_red_w''' & w''_red_w'''). 
-      shelve. Unshelve. simpl. lia.
-      epose proof (IH_v := IH _ _ _ _ _ _ _ v_red_v' v_red_v''). destruct IH_v as (v''' & v'_red_v''' & v''_red_v'''). 
-      shelve. Unshelve. simpl. lia.
+      try epose proof (IH_w := IH w ltac:(simpl; lia) _ _ _ _ _ w_red_w' w_red_w''); try destruct IH_w as (w''' & w'_red_w''' & w''_red_w'''). 
 
       do 4 eexists. exists (w''' <[ v''' ..]). split.
-      ++ eapply ortho_beta. 
-        +++ eauto using conv_sym, conv_trans. 
-        +++ eapply conv_in_ctx_conv. apply conv_ccons. eapply refl_ctx. auto. apply A_conv_A'. eauto using conv_sym, conv_trans.
-        +++ eapply ortho_conv_in_ctx. apply conv_ccons. eapply refl_ctx. auto. apply A_conv_A'. eapply ortho_conv. eauto. eauto using conv_sym, conv_trans.
-        +++ eapply ortho_conv. eauto. eauto.
-      ++ eapply ortho_subst_property. eapply (well_scons _ _ _ Γ l A). ssimpl. apply ortho_subst_id. auto. ssimpl. auto. eauto.
+      ++ eapply ortho_beta;  use_auto ; eauto using conv_sym, conv_trans. 
+        eapply (conv_in_ctx_conv (Γ ,, (l, A))). ctx_conv_auto. eauto using conv_sym, conv_trans.
+      ++ eapply ortho_subst_property. eapply (ortho_scons _ _ _ Γ l A). ssimpl. apply ortho_subst_id. auto. ssimpl. auto. eauto.
     
     (* beta x app-cong *)
     + admit. 
 
     (* beta x beta *)
-    + destruct t_red_t' as (A0 & B0 & w & w' & v' & u_eq & _ & _ & w_red_w' & v_red_v' & t'_eq).
-      rewrite t'_eq. clear t'_eq t'.
-      destruct t_red_t'' as (A0_ & B0_ & w_ & w'' & v'' & u_eq_ & _ & _ & w_red_w'' & v_red_v'' & t''_eq).
-      rewrite t''_eq. clear t''_eq t''.
+    + rewrite u_eq in *. clear u_eq u.
+      inversion u_eq_.  rewrite <- H2 in *. clear A_conv_A0_ B_conv_B0_ H0 H1 H2 u_eq_ w_ A0_ B0_.
 
-      rewrite u_eq in *. clear u_eq u.
-      inversion u_eq_.  rewrite <- H2 in *. clear H0 H1 H2 u_eq_ w_ A0_ B0_.
+      try epose proof (IH_w := IH w ltac:(simpl; lia) _ _ _ _ _ w_red_w' w_red_w''); try destruct IH_w as (w''' & w'_red_w''' & w''_red_w'''). 
 
-      epose proof (IH_w := IH _ _ _ _ _ _ _ w_red_w' w_red_w''). destruct IH_w as (w''' & w'_red_w''' & w''_red_w'''). 
-      shelve. Unshelve. simpl. lia.
-      epose proof (IH_v := IH _ _ _ _ _ _ _ v_red_v' v_red_v''). destruct IH_v as (v''' & v'_red_v''' & v''_red_v'''). 
-      shelve. Unshelve. simpl. lia.
-
-      do 4 eexists. exists (w''' <[ v''' .. ]).  split; eapply ortho_subst_property.
-      ++ eapply (well_scons _ _ _ Γ l A). ssimpl. apply ortho_subst_id. auto. ssimpl. auto.
-      ++ eauto.
-      ++ eapply (well_scons _ _ _ Γ l A). ssimpl. apply ortho_subst_id. auto. ssimpl. auto.
-      ++ eauto.
+      do 4 eexists. exists (w''' <[ v''' .. ]).  split; eapply ortho_subst_property; eauto. 
+      ++ eapply (ortho_scons _ _ _ Γ l A). ssimpl. apply ortho_subst_id. auto. ssimpl. auto.
+      ++ eapply (ortho_scons _ _ _ Γ l A). ssimpl. apply ortho_subst_id. auto. ssimpl. auto.
       
 
   (* Nat *)
@@ -545,20 +548,107 @@ Proof.
     ttinv t_red_t''. destruct t_red_t'' as (n'' & t''_eq & n_red_n'').
     rewrite t''_eq. clear t''_eq t''.
 
-    epose proof (IH_n := IH _ _ _ _ _ _ _ n_red_n' n_red_n''). destruct IH_n as (n''' & n'_red_n''' & n''_red_n'''). 
-    shelve. Unshelve. simpl. lia.
+    epose proof (IH_n := IH n ltac:(simpl; lia) _ _ _ _ _ n_red_n' n_red_n''). destruct IH_n as (n''' & n'_red_n''' & n''_red_n'''). 
 
     do 4 eexists. exists (succ n'''). split; eapply ortho_succ; eauto.
 
   (* rec *)
-  - admit.   
+  - rename t1 into P. rename t2 into p_zero. rename t3 into p_succ. rename t4 into n.
+    ttinv t_red_t'. ttinv t_red_t''. 
+    destruct t_red_t' as [(P' & p_zero' & p_succ' & n' & t'_eq & P_red_P' & p_zero_red_p_zero' & p_succ_red_p_succ' & n_red_n') 
+                        | [ (p_zero' & t'_eq & n_eq & p_zero_red_p_zero')
+                        | t_red_t']]; 
+    destruct t_red_t'' as [(P'' & p_zero'' & p_succ'' & n'' & t''_eq & P_red_P'' & p_zero_red_p_zero'' & p_succ_red_p_succ'' & n_red_n'') 
+                        | [ (p_zero'' & t''_eq & _n_eq & p_zero_red_p_zero'')
+                        | t_red_t'']]; 
+    try rewrite t'_eq in *; try clear t'_eq t'; try rewrite t''_eq in *; try clear t''_eq t'';
+    try epose proof (IH_P := IH P ltac:(simpl; lia) _ _ _ _ _ P_red_P' P_red_P''); try  destruct IH_P as (P''' & P'_red_P''' & P''_red_P''');
+    try epose proof (IH_p_zero := IH p_zero ltac:(simpl; lia) _ _ _ _ _ p_zero_red_p_zero' p_zero_red_p_zero'');
+    try destruct IH_p_zero as (p_zero''' & p_zero'_red_p_zero''' & p_zero''_red_p_zero''');
+    try epose proof (IH_p_succ := IH p_succ ltac:(simpl; lia) _ _ _ _ _ p_succ_red_p_succ' p_succ_red_p_succ'');
+    try destruct IH_p_succ as (p_succ''' & p_succ'_red_p_succ''' & p_succ''_red_p_succ''').
+    (* try epose proof (IH_n := IH n ltac:(simpl; lia) _ _ _ _ _ n_red_n' n_red_n''); try destruct IH_n as (n''' & n'_red_n''' & n''_red_n''').  *)
+
+
+    + epose proof (IH_n := IH n ltac:(simpl; lia) _ _ _ _ _ n_red_n' n_red_n''). destruct IH_n as (n''' & n'_red_n''' & n''_red_n'''). 
+
+      assert (Γ,, (ty 0, Nat) ⊢< Ax l > P : Sort l) as WtP. { apply ortho_validity in P_red_P' as H. destruct H. eauto. }
+      assert (⊢ (Γ,, (ty 0, Nat)),, (l, P)). {apply ctx_cons; eauto. apply ctx_cons; eauto using type_nat.  }
+    
+      do 4 eexists. exists (rec l P''' p_zero''' p_succ''' n'''). split; eapply ortho_rec; eauto; use_auto; eapply subst_ty; eauto using ortho_to_conv.
+      ++  eapply well_scons. ssimpl. admit. ssimpl. eauto using type_zero.
+      ++  eapply well_scons. ssimpl. admit. ssimpl. eapply type_succ. eapply (type_var _ _ _ Nat); eauto.
+      ++  eapply well_scons. ssimpl. admit. ssimpl. eauto using type_zero.
+      ++  eapply well_scons. ssimpl. admit. ssimpl. eapply type_succ. eapply (type_var _ _ _ Nat); eauto.
+    + rewrite _n_eq in *. clear n _n_eq. ttinv n_red_n'. rewrite n_red_n' in *. clear n' n_red_n'. 
+    
+    do 4 eexists. exists p_zero'''. split. 
+      ++ eapply ortho_rec_zero; eauto. apply ortho_validity in P_red_P'. destruct P_red_P'. eauto. admit. 
+        apply ortho_validity in p_succ_red_p_succ'. destruct p_succ_red_p_succ'. use_auto.
+        eapply subst_ty. 2:{eauto using ortho_to_conv. } apply well_scons. ssimpl. admit. ssimpl. apply type_succ. eapply (type_var _ _ _ Nat). 
+        admit. eauto.
+      ++ eauto.
+    + 
+
+
 
 Admitted.
 
 Require Import Coq.Relations.Relation_Operators.
 Require Import Coq.Relations.Relation_Definitions.
 
-Definition ortho_redd Γ l A := clos_refl_trans _ (fun t u => ortho_red Γ l t u A).
+Definition ortho_redd Γ l t u A := clos_refl_trans _ (fun t u => ortho_red Γ l t u A) t u.
 
-Definition ortho_equiv Γ l A := clos_refl_sym_trans _ (fun t u => ortho_red Γ l t u A).
+Definition ortho_equiv Γ l t u A := clos_refl_sym_trans _ (fun t u => ortho_red Γ l t u A) t u.
 
+
+Notation "Γ ⊢< l > t ⟹* t' : A" := (ortho_redd Γ l t t' A) (at level 50, l, t, t', A at next level).
+Notation "Γ ⊢< l > t ≈ t' : A" := (ortho_equiv Γ l t t' A) (at level 50, l, t, t', A at next level).
+
+Lemma conv_to_equiv Γ l t u A :
+  Γ ⊢< l > t ≡ u : A -> Γ ⊢< l > t ≈ u : A.
+Proof.
+Admitted.
+
+Corollary CR Γ l t u A :
+  Γ ⊢< l > t ≈ u : A ->
+  exists v, Γ ⊢< l > t ⟹* v : A /\ Γ ⊢< l > u ⟹* v : A.
+Proof.
+Admitted.
+
+Lemma reduce_pi Γ l l1 l2 A B T U :
+  Γ ⊢< l > Pi l1 l2 A B ⟹* T : U ->
+  exists A' B',
+  T = Pi l1 l2 A' B' /\
+  Γ ⊢< Ax l1 > A ⟹* A' : Sort l1 /\
+  Γ ,, (l1, A) ⊢< Ax l2 > B ⟹* B' : Sort l2.
+Proof.
+  intros pi_red_T.
+  dependent induction pi_red_T; try rename y into T.
+  - ttinv H. destruct H as (A' & B' & T_eq & _ & A_red & B_red & _). do 2 eexists. split; eauto. split; apply rt_step; eauto.
+  - exists A. exists B. split. reflexivity. split; apply rt_refl.
+  - destruct (IHpi_red_T1 l1 l2 A B eq_refl) as (A'' & B'' & T_eq & A_red & B_red). 
+    rewrite T_eq in *. clear T_eq T.
+    destruct (IHpi_red_T2 l1 l2 A'' B'' eq_refl) as (A''' & B''' & T_eq & A''_red & B''_red).
+    exists A'''. exists B'''. split. eauto. split. eapply rt_trans; eauto.
+    eapply rt_trans; eauto. use_auto.
+    admit.
+Admitted.
+
+
+Corollary pi_inj Γ l l0 l1 A B A' B' : 
+  Γ ⊢< l > Pi l0 l1 A B ≡ Pi l0 l1 A' B' : Sort (Ru l0 l1) -> 
+  Γ ⊢< Ax l0 > A ≡ A' : Sort l0 /\ Γ ,, (l0, A) ⊢< Ax l1 > B ≡ B' : Sort l1.
+Proof.
+  intro Pi_eq.
+  apply conv_to_equiv in Pi_eq.
+  apply CR in Pi_eq.
+  destruct Pi_eq as (v & Pi_red_1 & Pi_red_2).
+  apply reduce_pi in Pi_red_1.
+  destruct Pi_red_1 as (A0 & B0 & v_eq & A_redd_A0 & B_redd_B0).
+  apply reduce_pi in Pi_red_2.
+  destruct Pi_red_2 as (A1 & B1 & v_eq_ & A'_redd_A1 & B'_redd_B1).
+  rewrite v_eq in *. inversion v_eq_. rewrite H0 in *. rewrite H1 in *.
+  clear A0 B0 H0 H1 v_eq v.
+  admit.
+Admitted.
