theories/BasicMetaTheory.v
@@ -27,6 +27,10 @@ Admitted.
 Theorem subst : forall Γ l t u A Δ σ τ, Δ ⊢s σ ≡ τ : Γ -> Γ ⊢< l > t ≡ u : A -> Δ ⊢< l > t <[ σ ] ≡ u <[ τ ] : A <[ σ ].
 Admitted.
 
+Corollary subst_ty : forall Γ l t u l' Δ σ, Δ ⊢s σ : Γ -> Γ ⊢< l > t ≡ u : Sort l' -> Δ ⊢< l > t <[ σ ] ≡ u <[ σ ] : Sort l'.
+Admitted.
+
+
 Theorem conv_in_ctx_ty : forall Γ Δ l t A, ⊢ Γ ≡ Δ -> Γ ⊢< l > t : A -> Δ ⊢< l > t : A.
 Admitted.
 
